theories/TLCbuffer.v
@@ -685,3 +685,30 @@ Ltac nrapply H :=
   | notypeclasses refine (H _ _ _ _ _ _ _ _ _ _ _ _ _ _) ].
 
 
+
+
+(* ---------------------------------------------------------------------- *)
+(* LibWf *)
+
+From TLC Require Import LibWf.
+
+Ltac induction_wf_core_then IH E X cont ::=
+  let clearX tt :=
+    first [ clear X | fail 3 "the variable on which the induction is done appears in the hypotheses" ] in
+  first [ pattern X; 
+          first [ eapply (@well_founded_ind _ E)
+                | eapply (@well_founded_ind _ (E _))
+                | eapply (@well_founded_ind _ (E _ _))
+                | eapply (@well_founded_ind _ (E _ _ _))
+                | applys well_founded_ind (wf_measure E)  
+                | applys well_founded_ind E ];
+          clearX tt;
+          match goal with
+          | |- wf _ => auto with wf
+          | |- well_founded _ => change well_founded with wf; auto with wf
+          | |- _ => intros X IH; cont tt
+          end ].
+
+
+
+Global Arguments list_sub [A].
